Test/civl/async/lock-service.bpl
@@ -1,83 +1,145 @@
 // RUN: %boogie "%s" > "%t"
 // RUN: %diff "%s.expect" "%t"
-// XFAIL: *
+
+type {:pending_async}{:datatype} PA;
+function {:constructor} A_Callback(tid: Tid) : PA;
 
 type {:linear "tid"} Tid = int;
 
 const nil:Tid;
-var {:layer 0,2} l:Tid;
-var {:layer 0,4} x:int;
+var {:layer 0,4} l:Tid;
+var {:layer 0,5} x:int;
 
-procedure {:atomic}{:layer 4} Client_atomic ({:linear_in "tid"} tid:Tid)
+procedure {:atomic}{:layer 5} A_Client ()
 modifies x;
 {
   x := x + 1;
 }
-
-procedure {:yields}{:layer 3}{:refines "Client_atomic"} Client ({:linear_in "tid"} tid:Tid)
-requires {:layer 2} tid != nil;
+procedure {:refines "A_Client"} Client({:hide}{:linear_in "tid"} tid:Tid)
+requires {:layer 4} tid != nil;
 {
-  async call GetLockAbstract(tid);
+  call GetLockAndCallback(tid);
 }
 
-procedure {:left}{:layer 3} GetLockAbstract_atomic({:linear_in "tid"} tid:Tid)
+procedure {:atomic}{:layer 4} A_GetLockAndCallback' ({:linear_in "tid"} tid:Tid)
 modifies x;
 {
+  assert tid != nil;
   x := x + 1;
 }
 
-procedure {:yields}{:layer 2}{:refines "GetLockAbstract_atomic"} GetLockAbstract({:linear_in "tid"} tid:Tid)
-requires {:layer 2} tid != nil;
+procedure {:IS_invariant}{:layer 3} INV({:linear_in "tid"} tid:Tid) returns ({:pending_async "A_Callback"} PAs: [PA]int)
+modifies l, x;
 {
-  call GetLock(tid);
+  assert tid != nil;
+  assume l == nil;
+  PAs := MapConst(0);
+  if (*) {
+    l := tid;
+    PAs[A_Callback(tid)] := 1;
+  } else {
+    x := x + 1;
+  }
 }
 
-procedure {:left}{:layer 2} Callback_atomic ({:linear_in "tid"} tid:Tid)
-modifies l,x;
+procedure {:left}{:layer 3} A_Callback ({:linear_in "tid"} tid:Tid)
+modifies l, x;
 {
   assert tid != nil && l == tid;
   x := x + 1;
   l := nil;
 }
-
-procedure {:yields}{:layer 1}{:refines "Callback_atomic"} Callback ({:linear_in "tid"} tid:Tid)
+procedure {:yields}{:layer 2}{:refines "A_Callback"} Callback ({:linear_in "tid"} tid:Tid)
 {
   var tmp:int;
-  call tmp := read_x(tid);
-  call write_x(tmp+1, tid);
-  async call ReleaseLock(tid);
+  call tmp := read_x_lock(tid);
+  call write_x_lock(tmp+1, tid);
+  async call {:sync} ReleaseLock(tid);
 }
+
+procedure {:both}{:layer 2} A_read_x_lock ({:linear "tid"} tid:Tid) returns (v:int)
+{ assert tid != nil && l == tid; v := x; }
+procedure {:yields}{:layer 1}{:refines "A_read_x_lock"} read_x_lock ({:linear "tid"} tid:Tid) returns (v:int)
+{ call v := read_x(); }
+
+procedure {:both}{:layer 2} A_write_x_lock (v:int, {:linear "tid"} tid:Tid)
+modifies x;
+{ assert tid != nil && l == tid; x := v; }
+procedure {:yields}{:layer 1}{:refines "A_write_x_lock"} write_x_lock (v:int, {:linear "tid"} tid:Tid)
+{ call write_x(v); }
+
+procedure {:atomic}{:layer 1} A_read_x () returns (v:int)
+{ v := x; }
+procedure {:yields}{:layer 0}{:refines "A_read_x"} read_x () returns (v:int);
+
+procedure {:atomic}{:layer 1} A_write_x (v:int)
+modifies x;
+{ x := v; }
+procedure {:yields}{:layer 0}{:refines "A_write_x"} write_x (v:int);
 
 // -----------------------------------------------------------------------------
 
-procedure {:atomic}{:layer 1,2} GetLock_atomic ({:linear_in "tid"} tid:Tid)
+procedure {:atomic}{:layer 3}
+{:IS "A_GetLockAndCallback'","INV"}{:elim "A_Callback"}
+A_GetLockAndCallback ({:linear_in "tid"} tid:Tid)
+returns ({:pending_async "A_Callback"} PAs: [PA]int)
 modifies l;
 {
   assert tid != nil;
   assume l == nil;
   l := tid;
+  PAs := MapConst(0)[A_Callback(tid) := 1];
+}
+procedure {:yields}{:layer 2}{:refines "A_GetLockAndCallback"} GetLockAndCallback ({:linear_in "tid"} tid:Tid)
+{
+  call GetLock(tid);
   async call Callback(tid);
 }
 
-procedure {:left}{:layer 1} ReleaseLock_atomic ({:linear_in "tid"} tid:Tid)
+procedure {:atomic}{:layer 2} A_GetLock ({:linear "tid"} tid:Tid)
+modifies l;
+{
+  assert tid != nil;
+  assume l == nil;
+  l := tid;
+}
+procedure {:yields}{:layer 1}{:refines "A_GetLock"} GetLock ({:linear "tid"} tid:Tid)
+{
+  var success:bool;
+  while (true)
+  invariant {:yields} {:layer 1} true;
+  {
+    call success := cas_l(nil, tid);
+    if (success) {
+      return;
+    }
+  }
+}
+
+procedure {:left}{:layer 2} A_ReleaseLock ({:linear_in "tid"} tid:Tid)
 modifies l;
 {
   assert tid != nil && l == tid;
   l := nil;
 }
+procedure {:yields}{:layer 1}{:refines "A_ReleaseLock"} ReleaseLock ({:linear_in "tid"} tid:Tid)
+{
+  call write_l(nil);
+}
 
-procedure {:yields}{:layer 0}{:refines "GetLock_atomic"} GetLock ({:linear_in "tid"} tid:Tid);
-procedure {:yields}{:layer 0}{:refines "ReleaseLock_atomic"} ReleaseLock ({:linear_in "tid"} tid:Tid);
+procedure {:atomic} {:layer 1} A_cas_l (oldval:Tid, newval:Tid) returns (success:bool)
+modifies l;
+{
+  if (l == oldval) {
+    l := newval;
+    success := true;
+  } else {
+    success := false;
+  }
+}
+procedure {:yields}{:layer 0}{:refines "A_cas_l"} cas_l (oldval:Tid, newval:Tid) returns (success:bool);
 
-// -----------------------------------------------------------------------------
-
-procedure {:both}{:layer 1} read_x_atomic ({:linear "tid"} tid:Tid) returns (v:int)
-modifies x;
-{ assert tid != nil && l == tid; v := x; }
-
-procedure {:both}{:layer 1} write_x_atomic (v:int, {:linear "tid"} tid:Tid)
-modifies x;
-{ assert tid != nil && l == tid; x := v; }
-
-procedure {:yields}{:layer 0}{:refines "read_x_atomic"} read_x ({:linear "tid"} tid:Tid) returns (v:int);
-procedure {:yields}{:layer 0}{:refines "write_x_atomic"} write_x (v:int, {:linear "tid"} tid:Tid);
+procedure {:atomic}{:layer 1} A_write_l (v:Tid)
+modifies l;
+{ l := v; }
+procedure {:yields}{:layer 0}{:refines "A_write_l"} write_l (v:Tid);
