Test/civl/inductive-sequentialization/NoChoice.bpl
@@ -4,8 +4,8 @@
 var {:layer 0,2} x:int;
 
 type {:pending_async}{:datatype} PA;
-function {:pending_async "INC"}{:constructor} INC_PA() : PA;
-function {:pending_async "DEC"}{:constructor} DEC_PA() : PA;
+function {:constructor} INC() : PA;
+function {:constructor} DEC() : PA;
 
 function {:inline} NoPAs () : [PA]int
 { (lambda pa:PA :: 0) }
@@ -17,7 +17,7 @@ procedure {:atomic}{:layer 1}
 MAIN ()
 returns ({:pending_async "INC","DEC"} PAs:[PA]int)
 {
-  PAs := NoPAs()[INC_PA() := 1][DEC_PA() := 1];
+  PAs := NoPAs()[INC() := 1][DEC() := 1];
 }
 
 procedure {:atomic}{:layer 2}
@@ -31,8 +31,8 @@ returns ({:pending_async "INC","DEC"} PAs:[PA]int)
 modifies x;
 {
   PAs := NoPAs();
-  if (*) { PAs[INC_PA()] := 1; } else { x := x + 1; }
-  if (*) { PAs[DEC_PA()] := 1; } else { x := x - 1; }
+  if (*) { PAs[INC()] := 1; } else { x := x + 1; }
+  if (*) { PAs[DEC()] := 1; } else { x := x - 1; }
 }
 
 ////////////////////////////////////////////////////////////////////////////////
