Test/civl/pending-async-2.bpl
@@ -5,8 +5,8 @@ const n:int;
 axiom n > 0;
 
 type {:pending_async}{:datatype} PA;
-function {:pending_async "A"}{:constructor} A_PA() : PA;
-function {:pending_async "B"}{:constructor} B_PA() : PA;
+function {:constructor} A() : PA;
+function {:constructor} B() : PA;
 
 function {:inline} NoPAs () : [PA]int
 { (lambda pa:PA :: 0) }
@@ -19,7 +19,7 @@ procedure {:atomic}{:layer 1} B () {}
 procedure {:left}{:layer 1} C () returns ({:pending_async "A"} PAs:[PA]int)
 {
   // create undeclared pending async to B
-  PAs := NoPAs()[A_PA() := 1][B_PA() := 1];
+  PAs := NoPAs()[A() := 1][B() := 1];
 }
 
 procedure {:left}{:layer 1} D () returns ({:pending_async "A","B"} PAs:[PA]int)
