Test/civl/pending-async-linearity.bpl
@@ -4,8 +4,8 @@
 type {:linear "pid"} Pid = int;
 
 type {:pending_async}{:datatype} PA;
-function {:pending_async "A"}{:constructor} A_PA(pid:int) : PA;
-function {:pending_async "B"}{:constructor} B_PA(pid:int) : PA;
+function {:constructor} A(pid:int) : PA;
+function {:constructor} B(pid:int) : PA;
 
 function {:inline} NoPAs () : [PA]int
 { (lambda pa:PA :: 0) }
@@ -22,35 +22,35 @@ procedure {:atomic}{:layer 1}
 M0 (pid:int)
 returns ({:pending_async "A"} PAs:[PA]int)
 {
-  PAs := NoPAs()[A_PA(/* out of thin air ☠ */ pid) := 1];
+  PAs := NoPAs()[A(/* out of thin air ☠ */ pid) := 1];
 }
 
 procedure {:atomic}{:layer 1}
 M1 ({:linear_in "pid"} pid:int)
 returns ({:pending_async "A"} PAs:[PA]int)
 {
-  PAs := NoPAs()[A_PA(pid) := 1];
+  PAs := NoPAs()[A(pid) := 1];
 }
 
 procedure {:atomic}{:layer 1}
 M2 ({:linear "pid"} pid:int)
 returns ({:pending_async "A"} PAs:[PA]int)
 {
-  PAs := NoPAs()[A_PA(/* duplication ☠ */ pid) := 1];
+  PAs := NoPAs()[A(/* duplication ☠ */ pid) := 1];
 }
 
 procedure {:atomic}{:layer 1}
 M3 ({:linear_in "pid"} pid1:int, {:linear_in "pid"} pid2:int)
 returns ({:pending_async "A","B"} PAs:[PA]int)
 {
-  PAs := NoPAs()[A_PA(pid1) := 1][B_PA(pid2) := 1];
+  PAs := NoPAs()[A(pid1) := 1][B(pid2) := 1];
 }
 
 procedure {:atomic}{:layer 1}
 M4 ({:linear_in "pid"} pid1:int, {:linear_in "pid"} pid2:int)
 returns ({:pending_async "A","B"} PAs:[PA]int)
 {
-  PAs := NoPAs()[A_PA(pid1) := 1][B_PA(/* duplication ☠ */ pid1) := 1];
+  PAs := NoPAs()[A(pid1) := 1][B(/* duplication ☠ */ pid1) := 1];
 }
 
 procedure {:atomic}{:layer 1}
@@ -58,7 +58,7 @@ M5 ({:linear_in "pid"} pid:int)
 returns ({:linear "pid"} pid_out:int, {:pending_async "A"} PAs:[PA]int)
 {
   pid_out := pid;
-  PAs := NoPAs()[A_PA(/* duplication ☠ */ pid) := 1];
+  PAs := NoPAs()[A(/* duplication ☠ */ pid) := 1];
 }
 
 procedure {:atomic}{:layer 1}
@@ -66,7 +66,7 @@ M6 ({:linear_in "pid"} pid1:int, {:linear_in "pid"} pid2:int, {:linear_in "pid"}
 returns ({:linear "pid"} pid_out:int, {:pending_async "A","B"} PAs:[PA]int)
 {
   pid_out := pid3;
-  PAs := NoPAs()[A_PA(pid1) := 1][B_PA(pid2) := 1];
+  PAs := NoPAs()[A(pid1) := 1][B(pid2) := 1];
 }
 
 procedure {:atomic}{:layer 1}
@@ -74,7 +74,7 @@ M7 ({:linear_in "pid"} pid:[int]bool)
 returns ({:pending_async "A"} PAs:[PA]int)
 {
   assert pid == (lambda i:int :: 1 <= i && i <= 10);
-  PAs := NoPAs()[A_PA(5) := 1];
+  PAs := NoPAs()[A(5) := 1];
 }
 
 procedure {:atomic}{:layer 1}
@@ -82,5 +82,5 @@ M8 ({:linear_in "pid"} pid:[int]bool)
 returns ({:pending_async "A"} PAs:[PA]int)
 {
   assert pid == (lambda i:int :: 1 <= i && i <= 10);
-  PAs := NoPAs()[A_PA(/* out of thin air ☠ */ 0) := 1];
+  PAs := NoPAs()[A(/* out of thin air ☠ */ 0) := 1];
 }
