Test/civl/inductive-sequentialization/paxos/is.sh
@@ -1,6 +1,6 @@
 #!/bin/bash
 
-# RUN: %boogie -proverOpt:O:smt.random_seed=10 Paxos.bpl PaxosSeqAxioms.bpl PaxosActions.bpl PaxosAbstractions.bpl PaxosSeq.bpl > "%t"
+# RUN: %boogie -proverOpt:O:smt.random_seed=100 Paxos.bpl PaxosSeqAxioms.bpl PaxosActions.bpl PaxosAbstractions.bpl PaxosSeq.bpl > "%t"
 # RUN: %diff "%s.expect" "%t"
 
-boogie -proverOpt:O:smt.random_seed=10 $@ Paxos.bpl PaxosSeqAxioms.bpl PaxosActions.bpl PaxosAbstractions.bpl PaxosSeq.bpl
+boogie -proverOpt:O:smt.random_seed=100 $@ Paxos.bpl PaxosSeqAxioms.bpl PaxosActions.bpl PaxosAbstractions.bpl PaxosSeq.bpl
